lesson5, draft

lesson5.v
@@ -17,13 +17,142 @@ This is inline Coq code [fun x => x] and now some block Coq code
 
 #<div>#
 *)
-Check (fun n => 1 + n + 1).
+
+Lemma ex1 x : 0 * x = 0.
+by []. Qed.
+
+Lemma ex2 x : x * 0 = 0.
+Fail by [].
+Admitted.
+
+Module A.
+
+Inductive expr :=
+  | Zero
+  | Mult (x : expr) (y : expr)
+  | Extra (stuff : nat).
+
+Fixpoint simplify e :=
+  match e with
+  | Mult Zero x => Zero
+  | Mult x Zero => Zero
+  | y => y
+  end.
+
+Fixpoint interp e :=
+  match e with
+  | Zero => 0
+  | Mult x y => (interp x) * (interp y)
+  | Extra x => x
+  end.
+
+Lemma go e : interp e = interp (simplify e).
+have im a b : interp (Mult a b) = (interp a) * (interp b) by [].
+elim: e => //= - [//|x y Hxy|e He] [|a b Hab|f Hf]; by [ rewrite muln0 | rewrite -im ].
+Qed.
+
+
+Lemma ex3 x : x * 0 = 0.
+Proof.
+rewrite -[LHS]/(interp (Mult (Extra x) Zero)).
+rewrite go.
+rewrite /=.
+by [].
+Defined.
+
+Eval lazy delta [ex3] beta in ex3.
+
+End A.
+
+Module B.
+
+Inductive expr :=
+  | Zero
+  | Minus (x : expr) (y : expr)
+  | Extra (n : nat).
+
+  Fixpoint simplify e :=
+  match e with
+  | Minus (Extra x) (Extra y) =>
+       match eqn x y with true => Zero | _ => e end
+  | y => y
+  end.
+
+Fixpoint interp e :=
+  match e with
+  | Zero => 0
+  | Minus x y => (interp x) - (interp y)
+  | Extra x => x
+  end.
+
+Lemma go e : interp e = interp (simplify e).
+have im a b : interp (Minus a b) = (interp a) - (interp b) by [].
+elim: e => //= - [//|x y Hxy|e He] [|a b Hab|f Hf]; try by rewrite -im.
+by rewrite /=; case: eqnP => //= ->; rewrite subnn.
+Qed.
+
+
+Lemma ex3 x : x - x = 0.
+Proof.
+rewrite -[LHS]/(interp (Minus (Extra x) (Extra x))).
+rewrite go.
+rewrite /=.
+Abort.
+
+End B.
+
+Module C.
+
+Inductive expr :=
+  | Zero
+  | Minus (x : expr) (y : expr)
+  | Extra (n : nat).
+
+  Fixpoint simplify e :=
+  match e with
+  | Minus (Extra x) (Extra y) =>
+       match eqn x y with true => Zero | _ => e end
+  | y => y
+  end.
+
+Fixpoint interp e c :=
+  match e with
+  | Zero => 0
+  | Minus x y => (interp x c) - (interp y c)
+  | Extra x => nth 0 c x
+  end.
+
+Lemma go e ct : interp e ct = interp (simplify e) ct.
+have im a b c : interp (Minus a b) c = (interp a c) - (interp b c) by [].
+elim: e => //= - [//|x y Hxy|e He] [|a b Hab|f Hf]; try by rewrite -im.
+by rewrite /=; case: eqnP => //= ->; rewrite subnn.
+Qed.
+
+Lemma ex3 x : x - x = 0.
+Proof.
+rewrite -[LHS]/(interp (Minus (Extra 0) (Extra 0)) [::x]).
+rewrite go.
+rewrite /=.
+by [].
+Qed.
+
+
+(* 
+- computation is powerful on closed terms
+- proof size is constant
+
+*)
+
+
+
 (**
 #</div>#
 
 You cna also put latex math here
 
-#$$ \sum_{i=1}^n (i * 2 - 1) = n ^ 2 $$#
+#$$ \
+
+{i=1}^n (i * 2 - 1) = n ^ 2 $$#
 
 finally some notes, hover to unravel
 
